Dev fin

AbsTheorySyn.v
@@ -1,5 +1,4 @@
 Require Import List.
-Require Import Compare_dec.
 Require Import Omega.
 
 (******************************************************************************************)
@@ -19,9 +18,13 @@ Module Type TheorySig.
 (*The set of first-order terms*)
 Parameter foterm : Set.
 
-(*Lift term*)
+(*Lift is the recocation of free variables*)
 Parameter lift_trm_rec : foterm -> nat -> nat -> foterm.
 Definition lift_trm t n := lift_trm_rec t n 0.
+
+Axiom lift_trm0 : forall t, lift_trm t 0 = t.
+Axiom lift_trm_split : forall t n k, 
+  lift_trm_rec t (S n) k = lift_trm_rec (lift_trm_rec t n k) 1 k.
 
 (*Substitute term*)
 Parameter subst_trm_rec : foterm -> foterm -> nat -> foterm.
@@ -34,6 +37,22 @@ Definition subst_trm M N := subst_trm_rec M N 0.
 Parameter fv_trm_rec : foterm -> (*k*)nat -> list nat.
 Definition fv_trm t := fv_trm_rec t 0.
 
+Axiom in_S_fv_trm : forall t n k,
+  In (S n) (fv_trm_rec t k) <->
+  In n (fv_trm_rec t (S k)).
+
+Axiom in_fv_trm_lift : forall t n k k' k'',
+  In n (fv_trm_rec (lift_trm_rec t k' k'') (k+k'+k'')) <->
+  In n (fv_trm_rec t (k+k'')).
+
+Axiom in_fv_trm_subst_split : forall t n N k k',
+  In n (fv_trm_rec (subst_trm_rec t N k') (k+k')) ->
+  In n (fv_trm_rec N k) \/ In (S n) (fv_trm_rec t (k+k')).
+
+Axiom in_fv_trm_subst : forall t n N k k',
+  In (S n) (fv_trm_rec t (k+k')) ->
+  In n (fv_trm_rec (subst_trm_rec t N k') (k+k')).
+
 End TheorySig.
 
 
@@ -43,8 +62,9 @@ End TheorySig.
 (******************************************************************************************)
 Module FoLang (M : TheorySig).
 
-Import M.
+Export M.
 
+(*Fist order foformula*)
 Inductive foformula :=
 | eq_fotrm : foterm -> foterm -> foformula
 | TF   : foformula
@@ -56,6 +76,7 @@ Inductive foformula :=
 | fall : foformula -> foformula
 | exst : foformula -> foformula.
 
+(*Relication of the free variables of formula*)
 Fixpoint lift_fml_rec f n k:=
   match f with
     | eq_fotrm x y => eq_fotrm (lift_trm_rec x n k) (lift_trm_rec y n k)
@@ -71,6 +92,26 @@ Fixpoint lift_fml_rec f n k:=
 
 Definition lift_fml t n := lift_fml_rec t n 0.
 
+Lemma lift_fml_split : forall f n k, 
+  lift_fml_rec f (S n) k = lift_fml_rec (lift_fml_rec f n k) 1 k.
+induction f; trivial; unfold lift_fml in *; simpl; intros.
+ rewrite lift_trm_split with (t:=f).
+ rewrite lift_trm_split with (t:=f0); trivial.
+
+ rewrite IHf; trivial.
+
+ rewrite IHf1, IHf2; trivial.
+ 
+ rewrite IHf1, IHf2; trivial.
+
+ rewrite IHf1, IHf2; trivial.
+
+ rewrite IHf; trivial.
+
+ rewrite IHf; trivial.
+Qed.
+
+(*Substitution of formular*)
 Fixpoint subst_fml_rec f N n :=
   match f with
     | eq_fotrm x y => eq_fotrm (subst_trm_rec x N n) (subst_trm_rec y N n)
@@ -86,6 +127,7 @@ Fixpoint subst_fml_rec f N n :=
 
 Definition subst_fml f N := subst_fml_rec f N 0.
 
+(*Free variables of the formula : enjoy the same idea with the definiton on foterm*)
 Fixpoint fv_fml_rec f k : list nat :=
   match f with
     | eq_fotrm t1 t2 => (fv_trm_rec t1 k) ++ (fv_trm_rec t2 k)
@@ -101,22 +143,128 @@ Fixpoint fv_fml_rec f k : list nat :=
 
 Definition fv_fml f := fv_fml_rec f 0.
 
+Lemma in_S_fv_fml : forall f n k, 
+  In (S n) (fv_fml_rec f k) <-> In n (fv_fml_rec f (S k)).
+induction f; simpl; try reflexivity; trivial; intros; do 2 rewrite in_app_iff.
+ do 2 rewrite in_S_fv_trm; reflexivity.
+
+ rewrite IHf1, IHf2; reflexivity.
+
+ rewrite IHf1, IHf2; reflexivity.
+
+ rewrite IHf1, IHf2; reflexivity.
+Qed.
+
+Lemma in_fv_fml_lift : forall f n k k' k'',
+  In n (fv_fml_rec (lift_fml_rec f k' k'') (k+k'+k'')) <->
+  In n (fv_fml_rec f (k+k'')).
+induction f; simpl; intros; try reflexivity; trivial.
+ do 2 rewrite in_app_iff. do 2 rewrite in_fv_trm_lift; reflexivity.
+
+ do 2 rewrite in_app_iff. rewrite IHf1, IHf2; reflexivity.
+
+ do 2 rewrite in_app_iff. rewrite IHf1, IHf2; reflexivity.
+
+ do 2 rewrite in_app_iff. rewrite IHf1, IHf2; reflexivity.
+
+ replace (S (k + k'+ k'')) with (k + k' + S k'') by omega.
+ replace (S (k + k'')) with (k + S k'') by omega. apply IHf; trivial.
+
+ replace (S (k + k'+ k'')) with (k + k' + S k'') by omega.
+ replace (S (k + k'')) with (k + S k'') by omega. apply IHf; trivial.
+Qed.
+
+Lemma in_fv_fml_subst_split : forall g n N k k',
+  In n (fv_fml_rec (subst_fml_rec g N k') (k+k')) -> 
+  In n (fv_trm_rec N k) \/ In (S n) (fv_fml_rec g (k+k')).
+induction g; simpl; intros; try contradiction; trivial.
+ rewrite in_app_iff in H |- *.
+ destruct H as [H|H]; apply in_fv_trm_subst_split in H.
+  destruct H; [left|right; left]; trivial.
+  
+  destruct H; [left|right; right]; trivial.
+
+ apply IHg in H; trivial.
+ 
+ rewrite in_app_iff in H |- *. destruct H as [H|H]; [apply IHg1 in H|apply IHg2 in H].
+  destruct H; [left|right; left]; trivial.
+
+  destruct H; [left|right; right]; trivial.
+
+ rewrite in_app_iff in H |- *. destruct H as [H|H]; [apply IHg1 in H|apply IHg2 in H].
+  destruct H; [left|right; left]; trivial.
+
+  destruct H; [left|right; right]; trivial.
+
+ rewrite in_app_iff in H |- *. destruct H as [H|H]; [apply IHg1 in H|apply IHg2 in H].
+  destruct H; [left|right; left]; trivial.
+
+  destruct H; [left|right; right]; trivial.
+
+ replace (S (k + k')) with (k + S k') in H |- * by omega. apply IHg in H; trivial.
+
+ replace (S (k + k')) with (k + S k') in H |- * by omega. apply IHg in H; trivial.
+Qed.
+
+Lemma in_fv_fml_subst : forall f n N k k',
+  In (S n) (fv_fml_rec f (k+k')) ->
+  In n (fv_fml_rec (subst_fml_rec f N k') (k+k')).
+induction f; simpl; intros; trivial.
+ rewrite in_app_iff in H |- *.
+ destruct H; [left|right]; apply in_fv_trm_subst; trivial.
+
+ apply IHf; trivial.
+
+ rewrite in_app_iff in H |- *.
+ destruct H; [left; apply IHf1|right; apply IHf2]; trivial.
+
+ rewrite in_app_iff in H |- *.
+ destruct H; [left; apply IHf1|right; apply IHf2]; trivial.
+
+ rewrite in_app_iff in H |- *.
+ destruct H; [left; apply IHf1|right; apply IHf2]; trivial.
+
+ replace (S (k + k')) with (k + S k') in H |- * by omega. apply IHf; trivial.
+
+ replace (S (k + k')) with (k + S k') in H |- * by omega. apply IHf; trivial.
+Qed.
+
+(*Context is a list of foterm or formula*)
+(*In the list, None stands for foterm,*)
+(*and Some formula stands for the certain formular*)
+Definition HYP := list (option foformula).
+
+(*An well-typed term is the term with all free variables typed foterm*)
+Definition wf_trm (hyp : HYP) t := 
+  forall n, In n (fv_trm t) -> nth_error hyp n = Some None.
+
+(*An well-typed first order formula should contain merely free variables typed foterm*)
+Definition wf_fml (hyp : HYP) f := 
+  forall n, In n (fv_fml f) -> nth_error hyp n = Some None.
+
+Lemma wf_weakening : forall hyp t f',
+  wf_fml (t :: hyp) (lift_fml f' 1) ->
+  wf_fml hyp f'.
+intros; red in H |- *; intros. specialize H with (n:= S n).
+unfold fv_fml in H, H0. rewrite in_S_fv_fml in H.
+unfold lift_fml in H. replace 1 with (0+1+0) in H by omega.
+rewrite in_fv_fml_lift in H. simpl in H. apply H in H0; trivial.
+Qed.
+
 End FoLang.
-
-
 
 (******************************************************************************************)
 (*Theory axioms defines how valid fomula origns*)
 (******************************************************************************************)
 Module Type TheoryAx (M : TheorySig).
 
-Include FoLang(M).
+Include FoLang M.
 
 (*Theory Axioms*)
-Parameter ax_syn : list (option foformula) -> foformula -> Prop.
+Parameter ax_syn : HYP -> foformula -> Prop.
+Axiom ax_wf : forall hyp f, ax_syn hyp f -> wf_fml hyp f.
 
 End TheoryAx.
-
 
 (******************************************************************************************)
 (*Derivition rules defines how valid fomulas can be derived from the axioms*)
@@ -125,13 +273,7 @@ Module FoDeriv (M1 : TheorySig) (M2 : TheoryAx M1).
 
 Import M1 M2.
 
-Definition wf_trm (hyp:list (option foformula)) t := 
-  forall n, In n (fv_trm t) -> nth_error hyp n = Some None.
-
-Definition wf_fml (hyp:list (option foformula)) f := 
-  forall n, In n (fv_fml f) -> nth_error hyp n = Some None.
-
-Inductive deriv : list (option foformula) -> foformula -> Prop :=
+Inductive deriv : HYP -> foformula -> Prop :=
 | hyp_judge : forall f hyp n, 
   nth_error hyp n = Some (Some f) ->
   wf_fml hyp (lift_fml f (S n)) ->
@@ -170,27 +312,91 @@ Inductive deriv : list (option foformula) -> foformula -> Prop :=
   deriv hyp (exst f) -> 
   deriv (Some f::None::hyp) (lift_fml f1 2) -> deriv hyp f1.
 
+Lemma deriv_well_typed : forall hyp f, deriv hyp f -> wf_fml hyp f.
+induction 1; trivial.
+ apply ax_wf; trivial.
+
+ red; simpl; intros; contradiction.
+
+ red in IHderiv |- *. unfold fv_fml in IHderiv |- *. simpl in IHderiv |- *.
+ intros; apply IHderiv. rewrite app_nil_r; trivial.
+
+ red in IHderiv |- *. unfold fv_fml in IHderiv |- *. simpl in IHderiv |- *.
+ intros; apply IHderiv. rewrite app_nil_r in H0; trivial.
+
+ red in IHderiv1, IHderiv2 |- *. unfold fv_fml in IHderiv1, IHderiv2 |- *.
+ simpl; intros. apply in_app_iff in H1. 
+ destruct H1; [apply IHderiv1|apply IHderiv2]; trivial.
+
+ red in IHderiv |- *. unfold fv_fml in IHderiv |- *. simpl in IHderiv.
+ intros; apply IHderiv. rewrite in_app_iff; left; trivial.
+
+ red in IHderiv |- *. unfold fv_fml in IHderiv |- *. simpl in IHderiv.
+ intros; apply IHderiv. rewrite in_app_iff; right; trivial.
+
+ red in IHderiv, H0 |- *. unfold fv_fml in IHderiv, H0 |- *.
+ simpl; intros. apply in_app_iff in H1. 
+ destruct H1; [apply IHderiv|apply H0]; trivial.
+
+ red in IHderiv, H |- *. unfold fv_fml in IHderiv, H |- *.
+ simpl; intros. apply in_app_iff in H1. 
+ destruct H1; [apply H|apply IHderiv]; trivial.
+
+ apply wf_weakening in IHderiv2; trivial.
+
+ apply wf_weakening in IHderiv.
+ red in IHderiv, H |- *. unfold fv_fml in IHderiv, H |- *. simpl; intros.
+ rewrite in_app_iff in H1. destruct H1; [apply H in H1|apply IHderiv in H1]; trivial.
+
+ red in IHderiv1 |- *. unfold fv_fml in IHderiv1 |- *. intros; apply IHderiv1.
+ simpl; rewrite in_app_iff; right; trivial.
+
+ red in IHderiv |- *. unfold fv_fml in IHderiv |- *. simpl; intros.
+ rewrite <- in_S_fv_fml in H0. apply IHderiv in H0. simpl in H0; trivial.
+
+ red in IHderiv |- *. unfold fv_fml in IHderiv |- *. simpl; intros.
+ simpl in IHderiv. unfold subst_fml in H1.
+ replace 0 with (0+0) in H1 by omega. apply in_fv_fml_subst_split in H1.
+ destruct H1; [apply H in H1
+   |rewrite in_S_fv_fml in H1; simpl in H1; apply IHderiv in H1]; trivial.
+
+ red in IHderiv |- *. unfold fv_fml in IHderiv |- *. simpl in IHderiv |- *.
+ intros; apply IHderiv. rewrite <- in_S_fv_fml in H1.
+ unfold subst_fml. replace 0 with (0+0) in H1 |- * by omega.
+ apply in_fv_fml_subst; trivial.
+  
+ unfold lift_fml in IHderiv2. rewrite lift_fml_split in IHderiv2.
+ fold (lift_fml f1 1) in IHderiv2. fold (lift_fml (lift_fml f1 1) 1) in IHderiv2.
+ apply wf_weakening in IHderiv2. apply wf_weakening in IHderiv2; trivial.
+Qed. 
+
 End FoDeriv.
 
 
 (******************************************************************************************)
-(*This model defines the first-order theory with 3 parts :*)
-(*1. The first-order language defined above*)
-(*2. The axioms*)
+(*This model defines the first-order theory with 4 parts :*)
+(*1. The abstract signature of the theory*)
+(*2. The first-order language defined above*)
+(*3. The axioms defined abstractly*)
 (*3. Derivation rules*)
 (******************************************************************************************)
-Module Type TheorySyn (M : TheorySig) (MM : TheoryAx M).
 
-Include FoLang M.
-Include FoDeriv M MM.
+Module Type TheorySyn.
 
-Import M MM.
+(*Signature of the theory*)
+Declare Module sig : TheorySig.
+Export sig.
+(*Check foterm.*)
 
-(*Any derivable formula should well typed*)
-Parameter deriv_well_typed : forall hyp f, deriv hyp f -> wf_fml hyp f.
+(*First order language is included when defining abstract axioms*)
+Declare Module ax : TheoryAx sig.
+Export ax.
+(*Print foformula.*)
+(*Check ax_syn.*)
 
-Parameter wf_weakening : forall hyp t f',
-  wf_fml (t :: hyp) (lift_fml f' 1) ->
-  wf_fml hyp f'.
+(*Derivation rules are included now*)
+Include FoDeriv sig ax.
+(*Print deriv.*)
 
 End TheorySyn.
+
